src/Crypto/Digests.dfy
@@ -1,15 +1,16 @@
-include "../Util/StandardLibrary.dfy"
+include "../StandardLibrary/StandardLibrary.dfy"
 
 module {:extern "Digests"} Digests {
-  import opened StandardLibrary
+    import opened StandardLibrary
+    import opened UInt = StandardLibrary.UInt
 
-  datatype {:extern "HMAC_ALGORITHM"} HMAC_ALGORITHM = HmacSHA256 | HmacSHA384 | HmacNOSHA
+    datatype {:extern "HMAC_ALGORITHM"} HMAC_ALGORITHM = HmacSHA256 | HmacSHA384 | HmacNOSHA
   
-  // Hash length in octets, e.g. HashLength(SHA256) = 256 = 32 * 8
-  function {:axiom} HashLength(algorithm: HMAC_ALGORITHM): nat
-    ensures algorithm == HmacSHA256 ==> HashLength(algorithm) == 32
-    ensures algorithm == HmacSHA384 ==> HashLength(algorithm) == 48
+    // Hash length in octets, e.g. HashLength(SHA256) = 256 = 32 * 8
+    function {:axiom} HashLength(algorithm: HMAC_ALGORITHM): nat
+        ensures algorithm == HmacSHA256 ==> HashLength(algorithm) == 32
+        ensures algorithm == HmacSHA384 ==> HashLength(algorithm) == 48
 
-  function {:axiom} Hash(algorithm: HMAC_ALGORITHM, key: seq<byte>, message: seq<byte>): seq<byte>
-    ensures |Hash(algorithm, key, message)| == HashLength(algorithm)
+    function {:axiom} Hash(algorithm: HMAC_ALGORITHM, key: seq<uint8>, message: seq<uint8>): seq<uint8>
+        ensures |Hash(algorithm, key, message)| == HashLength(algorithm)
 }
