src/Crypto/EncryptionDefs.dfy
@@ -1,12 +1,14 @@
-include "../Util/StandardLibrary.dfy"
+include "../StandardLibrary/StandardLibrary.dfy"
 include "Cipher.dfy"
 
 module {:extern "EncDefs"} EncDefs {
     import C = Cipher
     import opened StandardLibrary
-    datatype {:extern "Msg"} Msg = Msg(m: seq<byte>)
-    datatype {:extern "EncryptionKey"} EncryptionKey = EK(k : seq<byte>)
-    datatype {:extern "DecryptionKey"} DecryptionKey = DK(k : seq<byte>)
-    datatype {:extern "MData"} MData = MD(md : seq<byte>) 
-    datatype {:extern "Ctx"} Ctx = Ctx(c : seq<byte>)
+    import opened UInt = StandardLibrary.UInt
+
+    datatype {:extern "Msg"} Msg = Msg(m: seq<uint8>)
+    datatype {:extern "EncryptionKey"} EncryptionKey = EK(k : seq<uint8>)
+    datatype {:extern "DecryptionKey"} DecryptionKey = DK(k : seq<uint8>)
+    datatype {:extern "MData"} MData = MD(md : seq<uint8>) 
+    datatype {:extern "Ctx"} Ctx = Ctx(c : seq<uint8>)
 }
