src/Crypto/GenBytes.dfy
@@ -1,14 +1,16 @@
-include "../Util/StandardLibrary.dfy"
+include "../StandardLibrary/StandardLibrary.dfy"
 
 module {:extern "RNGWrap"} RNG {
     import opened StandardLibrary
+    import opened UInt = StandardLibrary.UInt
+
     class {:extern} GenBytesClass {
-        method {:extern} GenUniformArray(i : uint16) returns (o : array<byte>) ensures o.Length == i as nat
-        method {:extern} GenUniformSeq(i : uint16) returns (o : seq<byte>) ensures |o| == i as nat
+        method {:extern} GenUniformArray(i : uint16) returns (o : array<uint8>) ensures o.Length == i as nat
+        method {:extern} GenUniformSeq(i : uint16) returns (o : seq<uint8>) ensures |o| == i as nat
         constructor {:extern} ()
     }
 
-    method GenBytes(i : uint16) returns (o : seq<byte>) ensures |o| == i as nat {
+    method GenBytes(i : uint16) returns (o : seq<uint8>) ensures |o| == i as nat {
         var x := new GenBytesClass();
         o := x.GenUniformSeq(i);
     }
