src/Util/UTF8.dfy
@@ -1,4 +1,4 @@
-include "StandardLibrary.dfy"
+include "../StandardLibrary/StandardLibrary.dfy"
 
 // Provides a function ValidUTF8 which checks if an array of bytes is a valid sequence of UTF8 code points.
 // Each code point of a UTF8 string is one of the following variants, ranging from one to four bytes:
@@ -7,31 +7,32 @@ include "StandardLibrary.dfy"
 // Case 3 : 1110xxxx 10xxxxxx 10xxxxxx
 // Case 4 : 11110xxx 10xxxxxx 10xxxxxx 10xxxxxx
 
-// The first byte of each code point is called the leading byte, while the rest are called continuation bytes.
+// The first uint8 of each code point is called the leading uint8, while the rest are called continuation bytes.
 
 // This does NOT perform any range checks on the values encoded.
 
 module UTF8 {
     import opened StandardLibrary
+    import opened UInt = StandardLibrary.UInt
 
     // Returns the value of the idx'th bit, from least to most significant bit (0- indexed)
-    function method bit_at (x: byte, idx: byte): bool
+    function method bit_at (x: uint8, idx: uint8): bool
     requires idx < 8
     {
     var w := x as bv8;
     (w >> idx) & 1 == 1
     }
 
-    // Checks if a[offset] is a valid continuation byte.
-    predicate method ValidUTF8Continuation (a : array<byte>, offset : nat)
+    // Checks if a[offset] is a valid continuation uint8.
+    predicate method ValidUTF8Continuation (a : array<uint8>, offset : nat)
         reads a
         requires a.Length > offset 
     {
             bit_at(a[offset], 7) && !bit_at(a[offset], 6)
     }
 
-    // Returns which leading byte is at a[offset], or 0 if it is not a leading byte.
-    function method CodePointCase (a : array<byte>, offset: nat)  : byte
+    // Returns which leading uint8 is at a[offset], or 0 if it is not a leading uint8.
+    function method CodePointCase (a : array<uint8>, offset: nat)  : uint8
         reads a
         requires offset < a.Length
     {
@@ -54,7 +55,7 @@ module UTF8 {
             1
     }
 
-    predicate method ValidUTF8_at (a : array<byte>, offset : nat)
+    predicate method ValidUTF8_at (a : array<uint8>, offset : nat)
         reads a 
         requires offset <= a.Length
         decreases (a.Length - offset)
@@ -83,7 +84,7 @@ module UTF8 {
             ValidUTF8_at(a, offset + 4)
     }
 
-    predicate method ValidUTF8 (a : array<byte>)
+    predicate method ValidUTF8 (a : array<uint8>)
         reads a
     {
         ValidUTF8_at(a, 0)
